If 

\begin{align*}
    \boldsymbol{P} = \begin{bmatrix}
        2 & 1 \\ 4 & 3
    \end{bmatrix} \\
    \boldsymbol{B} = \begin{bmatrix}
        1 & 2 \\ 2 & 3
    \end{bmatrix}
\end{align*}

compute $\left(\boldsymbol{PB}\right)^-1$.

\begin{solution}
    \begin{align*}
        \det\left(\boldsymbol{B}\right) = -1 \\
        \boldsymbol{B}^-1 = -1 \begin{bmatrix}
            3 & -2 \\
            -2 &  1
        \end{bmatrix} \\
        \boldsymbol{B}^-1 = \begin{bmatrix}
            -3 & 2 \\
            2 & -1
        \end{bmatrix}
    \end{align*}
    \begin{align*}
        (\boldsymbol{PB})^-1 = \boldsymbol{P}^-1\boldsymbol{B}^-1 \\
        (\boldsymbol{PB})^-1 = \begin{bmatrix}
            \frac{3}{2} & -\frac{1}{2} \\
            -2 & 1
        \end{bmatrix}
        \begin{bmatrix}
            -3 & 2 \\
            2 & -1
        \end{bmatrix}
        (\boldsymbol{PB})^-1 = \begin{bmatrix}
            -\frac{17}{2} & \frac{7}{2} \\
            5 & -2
        \end{bmatrix}
    \end{align*}
\end{solution}