Use the solutions of the characteristic equation to prove that $\lambda_1 + \lambda_2 = \tr(A)$.

\begin{solution}
    \begin{align*}
        \lambda^2 - \tr\left(\boldsymbol{A}\right)\lambda + \det\left(\boldsymbol{A}\right) = 0 \\
        \lambda &= \frac{\tr(\boldsymbol{A}) \pm \sqrt{\tr(\boldsymbol{A})^2 - 4\det(\boldsymbol{A})}}{2} \\
        \lambda_1 + \lambda_2 &= \tr(\boldsymbol{A}) + \sqrt{\tr(\boldsymbol{A})^2 - 4\det(\boldsymbol{A})} - \sqrt{\tr(\boldsymbol{A})^2 - 4\det(\boldsymbol{A})} \\
        \lambda_1 + \lambda_2 &= \tr(\boldsymbol{A})
    \end{align*}
\end{solution}