\begin{align*}
    \boldsymbol{A} &= \begin{bmatrix}
        1 & 2 \\
        3 & 2
    \end{bmatrix}
\end{align*}

\begin{solution}
    \begin{align*}
        \tr(\boldsymbol{A}) &= 3 \\
        \det(\boldsymbol{A}) &= -4 \\
        \lambda^2 - \tr(\boldsymbol{A})\lambda + \det(\boldsymbol{A}) &= 0 \\
        \lambda^2 - 3\lambda - 4 &= 0 \\
        (\lambda - 4)(\lambda + 1) &= 0 \\
        \lambda_1 &= -1 \\
        \lambda_2 &= 4 \\
        \\
        \boldsymbol{Av} &= \lambda\boldsymbol{v} \\
        \boldsymbol{Av}_1 &= \lambda_1\boldsymbol{v}_1 \\
        \begin{bmatrix}
            2 & 2 \\
            3 & 3
        \end{bmatrix}\boldsymbol{v}_1 &= \begin{bmatrix}
            0 \\ 0
        \end{bmatrix} \\
        \boldsymbol{v}_1 &= \begin{bmatrix}
            1 \\ -1
        \end{bmatrix} \\
        \begin{bmatrix}
            -3 & 2 \\
            3 & -2
        \end{bmatrix}\boldsymbol{v}_2 &= \begin{bmatrix}
            0 \\ 0
        \end{bmatrix} \\
        \boldsymbol{v}_2 &= \begin{bmatrix}
            2 \\ 3
        \end{bmatrix}
    \end{align*}
\end{solution}